src/program_proof/pav/merkle.v
@@ -12,7 +12,7 @@ Definition own_merkle ptr_tr entries : iProp Σ :=
   ∃ tr root,
   "%Htree" ∷ ⌜tree_to_map tr = entries⌝ ∗
   "Hnode" ∷ own_node root tr ∗
-  "Hroot" ∷ ptr_tr ↦[Tree :: "Root"] #root.
+  "Hroot" ∷ ptr_tr ↦[Tree :: "root"] #root.
 
 (* is_dig says that the tree with these entries has this digest. *)
 Definition is_dig entries dig : iProp Σ :=
